finish proof of ToPkv

lib/Buckets/KMBPKVOps.i.dfy
@@ -12,9 +12,20 @@ module KMBPKVOps {
   import KeyType
   import ValueType = ValueType`Internal
   import opened Sequences
+  import opened Maps
+  
+  predicate EncodableMessage(msg: KMB.Model.Messages.Message)
+  {
+    && msg.Define?
+  }
+
+  predicate EncodableMessageSeq(msgs: seq<KMB.Model.Messages.Message>)
+  {
+    && (forall i | 0 <= i < |msgs| :: EncodableMessage(msgs[i]))
+  }
 
   function messageSeq_to_bytestringSeq(msgs: seq<KMB.Model.Messages.Message>) : (result: seq<seq<byte>>)
-    requires forall i | 0 <= i < |msgs| :: msgs[i].Define?
+    requires EncodableMessageSeq(msgs)
     ensures |result| == |msgs|
     ensures forall i | 0 <= i < |result| :: result[i] == PKV.Message_to_bytestring(msgs[i])
   {
@@ -34,10 +45,18 @@ module KMBPKVOps {
     else
       bytestringSeq_to_MessageSeq(DropLast(strings)) + [ PKV.bytestring_to_Message(Last(strings)) ]
   }
+
+  lemma messageSeq_to_bytestringSeq_Additive(msgs1: seq<KMB.Model.Messages.Message>, msgs2: seq<KMB.Model.Messages.Message>)
+    requires EncodableMessageSeq(msgs1)
+    requires EncodableMessageSeq(msgs2)
+    ensures EncodableMessageSeq(msgs1 + msgs2)
+    ensures messageSeq_to_bytestringSeq(msgs1 + msgs2) == messageSeq_to_bytestringSeq(msgs1) + messageSeq_to_bytestringSeq(msgs2)
+  {
+  }
   
   method MessageArray_to_bytestringSeq(msgs: array<KMB.Model.Messages.Message>, nmsgs: uint64) returns (result: seq<seq<byte>>)
     requires nmsgs as nat <= msgs.Length
-    requires forall i | 0 <= i < nmsgs as int :: msgs[i].Define?
+    requires EncodableMessageSeq(msgs[..nmsgs])
     ensures result[..] == messageSeq_to_bytestringSeq(msgs[..nmsgs])
   {
     var aresult := new seq<byte>[nmsgs];
@@ -53,23 +72,88 @@ module KMBPKVOps {
 
     result := aresult[..i];
   }
+
+  predicate IsKeyMessageTree(node: KMB.Node)
+    reads node, node.repr
+  {
+    && KMB.WF(node)
+    && (forall k | k in KMB.Interpretation(node) :: PKV.ValidKeyByteString(k))
+    && (forall v | v in KMB.Interpretation(node).Values :: EncodableMessage(v))
+    && EncodableMessageSeq(KMB.ToSeq(node).1)
+  }
+
+  lemma IsKeyMessageTreeInheritance(node: KMB.Node, i: nat)
+    requires KMB.WF(node)
+    requires node.contents.Index?
+    requires IsKeyMessageTree(node)
+    requires i < node.contents.nchildren as nat
+    ensures IsKeyMessageTree(node.contents.children[i])
+  {
+    KMB.IOfChild(node, i);
+    var inode := KMB.I(node);
+    KMB.Model.ChildInterpretationSubMap(inode, i);
+    
+    var cs := KMB.Model.ToSeqChildren(inode.children).1;
+    calc {
+      KMB.ToSeq(node).1;
+      KMB.Model.ToSeq(KMB.I(node)).1;
+      KMB.Model.ToSeq(inode).1;
+      { KMB.Model.reveal_ToSeq(); }
+      Flatten(cs);
+    }
+
+    var csA := KMB.Model.ToSeqChildren(inode.children[..i]).1;
+    var csB := KMB.Model.ToSeqChildren(inode.children[i..i+1]).1;
+    var csC := KMB.Model.ToSeqChildren(inode.children[i+1..]).1;
+    calc {
+      KMB.Model.ToSeqChildren(inode.children).1;
+      {
+        KMB.Model.ToSeqChildrenAdditive(inode.children[..i], inode.children[i..]);
+        assert inode.children == inode.children[..i] + inode.children[i..];
+      }
+      csA + KMB.Model.ToSeqChildren(inode.children[i..]).1;
+      {
+        KMB.Model.ToSeqChildrenAdditive(inode.children[i..i+1], inode.children[i+1..]);
+        assert inode.children[i..] == inode.children[i..i+1] + inode.children[i+1..];
+      }
+      csA + csB + csC;
+    }
+
+    calc {
+      Flatten(cs);
+      { FlattenAdditive(csA + csB, csC); }
+      Flatten(csA + csB) + Flatten(csC);
+      { FlattenAdditive(csA, csB); }
+      Flatten(csA) + Flatten(csB) + Flatten(csC);
+    }
+
+    assert csB == [ KMB.Model.ToSeq(inode.children[i]).1 ];
+    assert Flatten(csB) == KMB.Model.ToSeq(inode.children[i]).1 by {
+      FlattenSingleton(KMB.Model.ToSeq(inode.children[i]).1);
+    }
+
+    assert forall m | m in KMB.ToSeq(node.contents.children[i]).1 :: m in KMB.ToSeq(node).1;
+    forall m | m in KMB.ToSeq(node.contents.children[i]).1
+      ensures EncodableMessage(m)
+    {
+    }
+  }
   
   method LeafFillDpkv(node: KMB.Node, dpkv: DPKV.DynamicPkv)
     requires KMB.WF(node)
     requires node.contents.Leaf?
     requires dpkv.WF()
     requires node.repr !! dpkv.Repr
-    requires forall k | k in KMB.Interpretation(node) :: |k| <= KeyType.MaxLen() as nat
-    requires forall v | v in KMB.Interpretation(node).Values :: v.Define?
+    requires IsKeyMessageTree(node)
     requires PKV.PSA.psaCanAppendSeq(dpkv.toPkv().keys, KMB.ToSeq(node).0)
-    requires forall i | 0 <= i < |KMB.ToSeq(node).1| :: KMB.ToSeq(node).1[i].Define?
     requires PKV.PSA.psaCanAppendSeq(dpkv.toPkv().messages, messageSeq_to_bytestringSeq(KMB.ToSeq(node).1))
     ensures dpkv.WF()
     ensures fresh(dpkv.Repr - old(dpkv.Repr))
-    ensures PKV.IKeys(dpkv.toPkv().keys) == old(PKV.IKeys(dpkv.toPkv().keys)) + KMB.ToSeq(node).0
-    ensures PKV.IMessages(dpkv.toPkv().messages) == old(PKV.IMessages(dpkv.toPkv().messages)) + KMB.ToSeq(node).1
+    ensures dpkv.toPkv().keys == PKV.PSA.psaAppendSeq(old(dpkv.toPkv().keys), KMB.ToSeq(node).0)
+    //ensures PKV.IKeys(dpkv.toPkv().keys) == old(PKV.IKeys(dpkv.toPkv().keys)) + KMB.ToSeq(node).0
+    ensures dpkv.toPkv().messages == PKV.PSA.psaAppendSeq(old(dpkv.toPkv().messages), messageSeq_to_bytestringSeq(KMB.ToSeq(node).1))
+    //ensures PKV.IMessages(dpkv.toPkv().messages) == old(PKV.IMessages(dpkv.toPkv().messages)) + KMB.ToSeq(node).1
     modifies dpkv.Repr
-    decreases node.height
   {
     var keys := node.contents.keys;
     var values := node.contents.values;
@@ -97,36 +181,262 @@ module KMBPKVOps {
     dpkv.messages.AppendSeq(messages);
     dpkv.Repr := {dpkv} + dpkv.keys.Repr + dpkv.messages.Repr;
 
+  }
+
+  lemma canAppendKeysIterate(pkv: PKV.Pkv, keyseqs: seq<seq<KMB.Model.Key>>)
+    requires PKV.WF(pkv)
+    requires 0 < |keyseqs|
+    requires PKV.PSA.psaCanAppendSeq(pkv.keys, Flatten(keyseqs))
+    ensures PKV.PSA.psaCanAppendSeq(pkv.keys, keyseqs[0])
+    ensures PKV.PSA.psaCanAppendSeq(PKV.PSA.psaAppendSeq(pkv.keys, keyseqs[0]), Flatten(keyseqs[1..]))
+  {
+    calc ==> {
+      PKV.PSA.psaCanAppendSeq(pkv.keys, Flatten(keyseqs));
+      { assert keyseqs == keyseqs[..1] + keyseqs[1..]; }
+      PKV.PSA.psaCanAppendSeq(pkv.keys, Flatten(keyseqs[..1] + keyseqs[1..]));
+      { FlattenAdditive(keyseqs[..1], keyseqs[1..]); }
+      PKV.PSA.psaCanAppendSeq(pkv.keys, Flatten(keyseqs[..1]) + Flatten(keyseqs[1..]));
+      { PKV.PSA.psaCanAppendSeqAdditive(pkv.keys, Flatten(keyseqs[..1]), Flatten(keyseqs[1..])); }
+      PKV.PSA.psaCanAppendSeq(pkv.keys, Flatten(keyseqs[..1]))
+        && PKV.PSA.psaCanAppendSeq(PKV.PSA.psaAppendSeq(pkv.keys, Flatten(keyseqs[..1])), Flatten(keyseqs[1..]));
+      {
+        reveal_Flatten();
+        assert keyseqs[0] == Last(keyseqs[..1]);
+        assert |DropLast(keyseqs[..1])| == 0;
+        assert [] + keyseqs[0] == keyseqs[0];
+      }
+      PKV.PSA.psaCanAppendSeq(pkv.keys, keyseqs[0])
+        && PKV.PSA.psaCanAppendSeq(PKV.PSA.psaAppendSeq(pkv.keys, keyseqs[0]), Flatten(keyseqs[1..]));
+    }
+  }
+  
+  lemma canAppendMessagesIterate(pkv: PKV.Pkv, msgseqs: seq<seq<KMB.Model.Messages.Message>>)
+    requires PKV.WF(pkv)
+    requires 0 < |msgseqs|
+    requires EncodableMessageSeq(Flatten(msgseqs))
+    requires PKV.PSA.psaCanAppendSeq(pkv.messages, messageSeq_to_bytestringSeq(Flatten(msgseqs)))
+    ensures EncodableMessageSeq(msgseqs[0])
+    ensures EncodableMessageSeq(Flatten(msgseqs[1..]))
+    ensures PKV.PSA.psaCanAppendSeq(pkv.messages, messageSeq_to_bytestringSeq(msgseqs[0]))
+    ensures PKV.PSA.psaCanAppendSeq(PKV.PSA.psaAppendSeq(pkv.messages, messageSeq_to_bytestringSeq(msgseqs[0])), messageSeq_to_bytestringSeq(Flatten(msgseqs[1..])))
+  {
     calc {
-      PKV.IMessages(dpkv.toPkv().messages);
-      bytestringSeq_to_MessageSeq(PKV.PSA.I(dpkv.toPkv().messages));
-      old(PKV.IMessages(dpkv.toPkv().messages)) + values[..nkeys];
+      Flatten(msgseqs);
+      {
+        assert msgseqs == msgseqs[..1] + msgseqs[1..];
+        FlattenAdditive(msgseqs[..1], msgseqs[1..]);
+      }
+      Flatten(msgseqs[..1]) + Flatten(msgseqs[1..]);
+      { assert msgseqs[..1] == [ msgseqs[0] ]; }
+      Flatten([ msgseqs[0] ]) + Flatten(msgseqs[1..]);
+      { FlattenSingleton(msgseqs[0]); }
+      msgseqs[0] + Flatten(msgseqs[1..]);
+    }
+    forall m | m in msgseqs[0]
+      ensures EncodableMessage(m)
+    {
+      assert m in Flatten(msgseqs);
+    }
+    forall m | m in Flatten(msgseqs[1..])
+      ensures EncodableMessage(m)
+    {
+      assert m in Flatten(msgseqs);
+    }
+
+    messageSeq_to_bytestringSeq_Additive(msgseqs[0], Flatten(msgseqs[1..]));
+    PKV.PSA.psaCanAppendSeqAdditive(pkv.messages, messageSeq_to_bytestringSeq(msgseqs[0]), messageSeq_to_bytestringSeq(Flatten(msgseqs[1..])));
+  }
+  
+  method IndexFillDpkv(node: KMB.Node, dpkv: DPKV.DynamicPkv)
+    requires KMB.WF(node)
+    requires node.contents.Index?
+    requires dpkv.WF()
+    requires node.repr !! dpkv.Repr
+    requires IsKeyMessageTree(node)
+    requires PKV.PSA.psaCanAppendSeq(dpkv.toPkv().keys, KMB.ToSeq(node).0)
+    requires PKV.PSA.psaCanAppendSeq(dpkv.toPkv().messages, messageSeq_to_bytestringSeq(KMB.ToSeq(node).1))
+    ensures dpkv.WF()
+    ensures fresh(dpkv.Repr - old(dpkv.Repr))
+    ensures dpkv.toPkv().keys == PKV.PSA.psaAppendSeq(old(dpkv.toPkv().keys), KMB.ToSeq(node).0)
+    ensures dpkv.toPkv().messages == PKV.PSA.psaAppendSeq(old(dpkv.toPkv().messages), messageSeq_to_bytestringSeq(KMB.ToSeq(node).1))
+    modifies dpkv.Repr
+    decreases node.height, 0
+  {
+    var children := node.contents.children;
+    var nchildren := node.contents.nchildren;
+
+    assert KMB.WFShapeChildren(children[..nchildren], node.repr, node.height);
+    ghost var inode := KMB.I(node);
+    ghost var ichildren := inode.children;
+    forall i | 0 <= i < |ichildren|
+      ensures ichildren[i] == KMB.IChildren(children[..nchildren], node.height)[i]
+    {
+      KMB.IOfChild(node, i);
+    }
+    assert ichildren == KMB.IChildren(children[..nchildren], node.height);
+    ghost var childSeqs := KMB.Model.ToSeqChildren(ichildren);
+    assert forall i | 0 <= i < |childSeqs.0| :: childSeqs.0[i] == KMB.ToSeq(children[i]).0 by {
+      KMB.Model.reveal_ToSeq();
+    }
+    assert forall i | 0 <= i < |childSeqs.1| :: childSeqs.1[i] == KMB.ToSeq(children[i]).1 by {
+      KMB.Model.reveal_ToSeq();
+    }
+
+    assert Flatten(childSeqs.0) == KMB.ToSeq(node).0 by {
+      KMB.reveal_I();
+      KMB.Model.reveal_ToSeq();
+    }
+    assert Flatten(childSeqs.1) == KMB.ToSeq(node).1 by {
+      KMB.reveal_I();
+      KMB.Model.reveal_ToSeq();
+    }
+    assert EncodableMessageSeq(Flatten(childSeqs.1));
+    forall i | 0 <= i <= nchildren
+      ensures EncodableMessageSeq(Flatten(childSeqs.1[..i]))
+      ensures EncodableMessageSeq(Flatten(childSeqs.1[i..]))
+    {
+      FlattenAdditive(childSeqs.1[..i], childSeqs.1[i..]);
+      assert childSeqs.1 == childSeqs.1[..i] + childSeqs.1[i..];
+      assert forall m | m in Flatten(childSeqs.1) :: EncodableMessage(m);
+    }
+
+    ghost var oldpkvkeys := old(dpkv.toPkv().keys);
+    ghost var oldpkvmsgs := old(dpkv.toPkv().messages);
+
+    forall i | 0 <= i <= nchildren
+      ensures PKV.PSA.psaCanAppendSeq(oldpkvkeys, Flatten(childSeqs.0[..i]))
+      ensures PKV.PSA.psaCanAppendSeq(oldpkvmsgs, messageSeq_to_bytestringSeq(Flatten(childSeqs.1[..i])))
+    {
+      FlattenAdditive(childSeqs.0[..i], childSeqs.0[i..]);
+      assert childSeqs.0 == childSeqs.0[..i] + childSeqs.0[i..];
+      PKV.PSA.psaCanAppendSeqAdditive(oldpkvkeys, Flatten(childSeqs.0[..i]), Flatten(childSeqs.0[i..]));
+
+      FlattenAdditive(childSeqs.1[..i], childSeqs.1[i..]);
+      assert childSeqs.1 == childSeqs.1[..i] + childSeqs.1[i..];
+      messageSeq_to_bytestringSeq_Additive(Flatten(childSeqs.1[..i]), Flatten(childSeqs.1[i..]));
+      PKV.PSA.psaCanAppendSeqAdditive(oldpkvmsgs, messageSeq_to_bytestringSeq(Flatten(childSeqs.1[..i])),
+        messageSeq_to_bytestringSeq(Flatten(childSeqs.1[i..])));
+    }
+    
+    var i: uint64 := 0;
+
+    while i < nchildren
+      invariant i <= nchildren
+      invariant dpkv.WF()
+      invariant fresh(dpkv.Repr - old(dpkv.Repr))
+      
+      invariant dpkv.toPkv().keys == PKV.PSA.psaAppendSeq(oldpkvkeys, Flatten(childSeqs.0[..i]))
+      invariant PKV.PSA.psaCanAppendSeq(dpkv.toPkv().keys, Flatten(childSeqs.0[i..]))
+
+      invariant dpkv.toPkv().messages == PKV.PSA.psaAppendSeq(oldpkvmsgs, messageSeq_to_bytestringSeq(Flatten(childSeqs.1[..i])))
+      invariant PKV.PSA.psaCanAppendSeq(dpkv.toPkv().messages, messageSeq_to_bytestringSeq(Flatten(childSeqs.1[i..])))
+    {
+      assert KMB.WF(children[i]);
+      assert dpkv.WF();
+      assert children[i].repr !! dpkv.Repr;
+
+      IsKeyMessageTreeInheritance(node, i as nat);
+      assert IsKeyMessageTree(children[i]);
+
+      canAppendKeysIterate(dpkv.toPkv(), childSeqs.0[i..]);
+      canAppendMessagesIterate(dpkv.toPkv(), childSeqs.1[i..]);
+
+      ghost var prekeys := dpkv.toPkv().keys;
+      ghost var premsgs := dpkv.toPkv().messages;
+      
+      FillDpkv(children[i], dpkv);
+      
+      calc {
+        dpkv.toPkv().keys;
+        PKV.PSA.psaAppendSeq(prekeys, KMB.ToSeq(children[i]).0);
+        PKV.PSA.psaAppendSeq(PKV.PSA.psaAppendSeq(oldpkvkeys, Flatten(childSeqs.0[..i])), KMB.ToSeq(children[i]).0);
+        { PKV.PSA.psaAppendSeqAdditive(oldpkvkeys, Flatten(childSeqs.0[..i]), KMB.ToSeq(children[i]).0); }
+        PKV.PSA.psaAppendSeq(oldpkvkeys, Flatten(childSeqs.0[..i]) + KMB.ToSeq(children[i]).0);
+        PKV.PSA.psaAppendSeq(oldpkvkeys, Flatten(childSeqs.0[..i]) + childSeqs.0[i]);
+        { FlattenSingleton(childSeqs.0[i]); }
+        PKV.PSA.psaAppendSeq(oldpkvkeys, Flatten(childSeqs.0[..i]) + Flatten([ childSeqs.0[i] ]));
+        { FlattenAdditive(childSeqs.0[..i], [ childSeqs.0[i] ]); }
+        PKV.PSA.psaAppendSeq(oldpkvkeys, Flatten(childSeqs.0[..i] + [ childSeqs.0[i] ]));
+        { assert childSeqs.0[..i+1] == childSeqs.0[..i] + [ childSeqs.0[i] ]; }
+        PKV.PSA.psaAppendSeq(oldpkvkeys, Flatten(childSeqs.0[..i+1]));
+      }
+
+    
+      calc {
+        dpkv.toPkv().messages;
+        PKV.PSA.psaAppendSeq(premsgs, messageSeq_to_bytestringSeq(KMB.ToSeq(children[i]).1));
+        PKV.PSA.psaAppendSeq(premsgs, messageSeq_to_bytestringSeq(childSeqs.1[i]));
+        PKV.PSA.psaAppendSeq(PKV.PSA.psaAppendSeq(oldpkvmsgs, messageSeq_to_bytestringSeq(Flatten(childSeqs.1[..i]))),
+                                                              messageSeq_to_bytestringSeq(childSeqs.1[i]));
+        { PKV.PSA.psaAppendSeqAdditive(oldpkvmsgs, messageSeq_to_bytestringSeq(Flatten(childSeqs.1[..i])),
+                                                   messageSeq_to_bytestringSeq(childSeqs.1[i])); }
+        PKV.PSA.psaAppendSeq(oldpkvmsgs, messageSeq_to_bytestringSeq(Flatten(childSeqs.1[..i])) +
+                                         messageSeq_to_bytestringSeq(childSeqs.1[i]));
+        { messageSeq_to_bytestringSeq_Additive(Flatten(childSeqs.1[..i]), childSeqs.1[i]); }
+        PKV.PSA.psaAppendSeq(oldpkvmsgs, messageSeq_to_bytestringSeq(Flatten(childSeqs.1[..i]) + childSeqs.1[i]));
+        { FlattenSingleton(childSeqs.1[i]); }
+        PKV.PSA.psaAppendSeq(oldpkvmsgs, messageSeq_to_bytestringSeq(Flatten(childSeqs.1[..i]) + Flatten([ childSeqs.1[i] ])));
+        { FlattenAdditive(childSeqs.1[..i], [ childSeqs.1[i] ]); }
+        PKV.PSA.psaAppendSeq(oldpkvmsgs, messageSeq_to_bytestringSeq(Flatten(childSeqs.1[..i] + [ childSeqs.1[i] ])));
+        { assert childSeqs.1[..i+1] == childSeqs.1[..i] + [ childSeqs.1[i] ]; }
+        PKV.PSA.psaAppendSeq(oldpkvmsgs, messageSeq_to_bytestringSeq(Flatten(childSeqs.1[..i+1])));
+      }
+      
+      i := i + 1;
+    }
+
+    calc {
+      dpkv.toPkv().keys;
+      PKV.PSA.psaAppendSeq(oldpkvkeys, Flatten(childSeqs.0[..i]));
+      { assert childSeqs.0[..i] == childSeqs.0; }
+      PKV.PSA.psaAppendSeq(old(dpkv.toPkv().keys), KMB.ToSeq(node).0);
+    }
+    calc {
+      dpkv.toPkv().messages;
+      PKV.PSA.psaAppendSeq(oldpkvmsgs, messageSeq_to_bytestringSeq(Flatten(childSeqs.1[..i])));
+      { assert childSeqs.1[..i] == childSeqs.1; }
+      PKV.PSA.psaAppendSeq(old(dpkv.toPkv().messages), messageSeq_to_bytestringSeq(KMB.ToSeq(node).1));
     }
   }
 
-  // } else {
-  //   assume false;
-  //   while i < node.contents.nchildren
-  //     invariant i <= node.contents.nchildren
-  //     invariant dpkv.WF()
-  //     invariant fresh(dpkv.Repr - old(dpkv.Repr))
-  //   {
-  //     KMB.IOfChild(node, i as int);
-  //     assert KMB.WFShapeChildren(node.contents.children[..node.contents.nchildren], node.repr, node.height);
-  //     FillDpkv(node.contents.children[i], dpkv);
-  //     i := i + 1;
-  //   }
-  // }
+  method FillDpkv(node: KMB.Node, dpkv: DPKV.DynamicPkv)
+    requires KMB.WF(node)
+    requires dpkv.WF()
+    requires node.repr !! dpkv.Repr
+    requires IsKeyMessageTree(node)
+    requires PKV.PSA.psaCanAppendSeq(dpkv.toPkv().keys, KMB.ToSeq(node).0)
+    requires PKV.PSA.psaCanAppendSeq(dpkv.toPkv().messages, messageSeq_to_bytestringSeq(KMB.ToSeq(node).1))
+    ensures dpkv.WF()
+    ensures fresh(dpkv.Repr - old(dpkv.Repr))
+    ensures dpkv.toPkv().keys == PKV.PSA.psaAppendSeq(old(dpkv.toPkv().keys), KMB.ToSeq(node).0)
+    ensures dpkv.toPkv().messages == PKV.PSA.psaAppendSeq(old(dpkv.toPkv().messages), messageSeq_to_bytestringSeq(KMB.ToSeq(node).1))
+    modifies dpkv.Repr
+    decreases node.height, 1
+  {
+    if node.contents.Leaf? {
+      LeafFillDpkv(node, dpkv);
+    } else {
+      IndexFillDpkv(node, dpkv);
+    }
+  }
+  
 
   method ToPkv(node: KMB.Node) returns (pkv: DPKV.PKV.Pkv)
     requires KMB.WF(node)
+    requires IsKeyMessageTree(node)
+    requires PKV.PSA.psaCanAppendSeq(PKV.PSA.EmptyPsa(), KMB.ToSeq(node).0)
+    requires PKV.PSA.psaCanAppendSeq(PKV.PSA.EmptyPsa(), messageSeq_to_bytestringSeq(KMB.ToSeq(node).1))
     ensures DPKV.PKV.WF(pkv)
+    ensures PKV.IKeys(pkv.keys) == KMB.ToSeq(node).0
+    ensures PKV.PSA.I(pkv.messages) == messageSeq_to_bytestringSeq(KMB.ToSeq(node).1)
   {
-    assume false;
+    KMB.Model.ToSeqLength(KMB.I(node));
     var nelts: uint64 := KMBBOps.CountElements(node);
-    var cap := DPKV.Capacity(nelts as uint32, (nelts * KeyType.MaxLen()) as uint32, (nelts * ValueType.MaxLen()) as uint32);
+    var keydatasize := if nelts * KeyType.MaxLen() <= 0xffff_ffff then (nelts * KeyType.MaxLen()) as uint32 else 0xffff_ffff;
+    var msgdatasize := if nelts * ValueType.MaxLen() <= 0xffff_ffff then (nelts * ValueType.MaxLen()) as uint32 else 0xffff_ffff;
+    var cap := DPKV.Capacity(nelts as uint32, keydatasize, msgdatasize);
     var dpkv := new DPKV.DynamicPkv.PreSized(cap);
-    //FillDpkv(node, dpkv);
+    FillDpkv(node, dpkv);
     pkv := dpkv.toPkv();
   }
 
